compiler/bytecode/bytecodeTerminationScript.sml
@@ -1,5 +1,11 @@
-open HolKernel boolLib bossLib BytecodeTheory
+open HolKernel Defn boolLib bossLib BytecodeTheory LabelsTheory lcsymtacs
 val _ = new_theory"bytecodeTermination"
+
+fun register name (def,ind) = let
+  val _ = save_thm(name^"_def", def)
+  val _ = save_thm(name^"_ind", ind)
+  val _ = computeLib.add_persistent_funs [name^"_def"]
+in (def,ind) end
 
 val _ = save_thm ("bc_fetch_aux_def", bc_fetch_aux_def);
 val _ = export_rewrites["bc_fetch_aux_def"];
@@ -23,5 +29,15 @@ val _ = export_rewrites["is_Label_def","bool_to_tag_def","bool_to_val_def",
                         "unit_tag_def","unit_val_def","closure_tag_def",
                         "block_tag_def"];
 val _ = Parse.overload_on("next_addr", ``λil ls. SUM (MAP (SUC o il) (FILTER ($~ o is_Label) ls))``)
+
+val _ = register "calculate_labels" (
+  tprove_no_defn ((calculate_labels_def,calculate_labels_ind),
+  WF_REL_TAC `measure (LENGTH o SND o SND o SND o SND)` >> rw[]))
+
+val _ = register "replace_labels" (
+  tprove_no_defn ((replace_labels_def,replace_labels_ind),
+  WF_REL_TAC `measure (LENGTH o SND o SND)` >> rw[]))
+
+val _ = export_rewrites["CompilerLib.the_def","CompilerLib.fapply_def"]
 
 val _ = export_theory()
